theories/ycombinator.v
@@ -1,0 +1,82 @@
+From iris.proofmode Require Import base tactics classes.
+From diris Require Import langdef langlemmas.
+
+Section ycombinator.
+  (* We define the y-combinator for creating recursive functions t1 -> t2. *)
+  Variable t1 t2 : type.
+
+  Definition gT := UFunT t1 t2.
+  Definition fT := UFunT gT gT.
+  CoFixpoint xT := UFunT xT gT.
+
+  Lemma unfold_xT : xT = UFunT xT gT.
+    by rewrite <-type_id_id at 1.
+  Qed.
+
+  Definition y1 := ULam "x" (UApp (Var "f") (ULam "v" (UApp (UApp (Var "x") (Var "x")) (Var "v")))).
+  Definition y := ULam "f" (UApp y1 y1).
+
+  Lemma Var_typed' x xT : typed {[x := xT]} (Var x) xT.
+  Proof.
+    replace {[x := xT]} with (∅ ∪ {[x := xT]} : envT) by rewrite left_id //.
+    eapply Var_typed; eauto.
+    eapply Γunrestricted_empty.
+  Qed.
+
+  Lemma Γunrestricted_singleton x xT : unrestricted xT -> Γunrestricted {[x := xT]}.
+  Proof.
+    intros ???. destruct (decide (x = x0)); subst.
+    - rewrite lookup_singleton. intros. simplify_eq. done.
+    - rewrite lookup_singleton_ne; eauto. intros. simplify_eq.
+  Qed.
+
+
+  Lemma singleton_disj x y xT yT :
+    String.eqb x y = false ∨ (xT = yT ∧ unrestricted xT) -> disj {[x := xT]} {[y := yT]}.
+  Proof.
+    intros ??????.
+    eapply lookup_singleton_Some in H0 as [].
+    eapply lookup_singleton_Some in H1 as [].
+    subst. rewrite String.eqb_refl in H.
+    destruct H; simplify_eq. destruct H; subst. eauto.
+  Qed.
+
+  Lemma fT_unrestricted : unrestricted fT.
+  Proof. constructor. Qed.
+  Lemma xT_unrestricted : unrestricted xT.
+    rewrite <-type_id_id. constructor.
+  Qed.
+
+  Ltac check := eauto using Γunrestricted_singleton, Γunrestricted_empty, fT_unrestricted, xT_unrestricted, singleton_disj.
+
+  Lemma ctx_dup (Γ : envT) : Γ = Γ ∪ Γ.
+  Proof.
+    eapply map_eq. intro.
+    rewrite lookup_union. destruct (_!!_); eauto.
+  Qed.
+
+  Lemma y1_typed : typed {[ "f" := fT ]} y1 (UFunT xT gT).
+  Proof.
+    unfold y1.
+    eapply ULam_typed; check.
+    eapply UApp_typed; check.
+    - eapply Var_typed'.
+    - eapply ULam_typed; check.
+      eapply UApp_typed; check.
+      + rewrite ->ctx_dup at 1.
+        eapply UApp_typed; check.
+        * rewrite ->unfold_xT at 1. eapply Var_typed'.
+        * eapply Var_typed'.
+      + eapply Var_typed'.
+  Qed.
+
+  Lemma y_typed : typed ∅ y (UFunT fT gT).
+  Proof.
+    unfold y.
+    eapply ULam_typed; check.
+    rewrite left_id. rewrite ->ctx_dup at 1.
+    eapply UApp_typed; check.
+    - eapply y1_typed.
+    - rewrite unfold_xT. eapply y1_typed.
+  Qed.
+End ycombinator.
